---
    print_background: true
    export_on_save:
        html: true
    puppeteer:
        format: "Letter"
        timeout: 3000
---

$$
    % Differentials d[something]/d[something]
    \gdef\diff#1#2{\frac{\mathrm{d}#1}{\mathrm{d}#2}}
    % Shortcut for dy/dx
    \gdef\dydx{\diff{y}{x}}
	% Shortcut for "not implies"
    \gdef\nimplies{\;\;\;\not\nobreak\!\!\!\!\implies\;}
$$

# 3.6 â€” Derivatives of Composite Functions

<div><note>

$$
f(x) = (3x - 4)^2 \nimplies f'(x) = 2(3x - 4)
$$

</note></div>

In general, if $h$ is a composite function of $f$ and $g$:

$$
h(x) = f(g(x)).
$$

Then,
$$
h'(x) \neq f'(g(x)).
$$

Instead, in order to find the derivatives of composite functions, we need to use the **chain rule**.

# Chain rule

<div><def>

Let $h$, $f$, and $g$ be functions where $h(x) = f(g(x))$, such that $f$ and $g$ are differentiable.

Then, the **chain rule** states: $h'(x) = f'(g(x)) \cdot g'(x)$.

In short,
$$
h(x) = f(g(x)) \implies h'(x) = f'(g(x)) \cdot g'(x)
$$

</def></div>

<div><eg>

Let $h(x) = (3x - 4)^2$. Find $h'(x)$.

Notice that $h$ is a composite function made up of two other functions.

* Let's call the "outer" function $f$, where $f(x) = x^2$.
* And the inner $g$, where $g(x) = 3x - 4$.

Then, $h(x) = f(g(x)) = (3x - 4)^2$.

Using the chain rule, we have that $h'(x) = f'(g(x)) \cdot g'(x)$.

$$
\begin{aligned}
    h'(x) &= f'(g(x)) \cdot g'(x) \\
    &= 2(3x - 4) \cdot 3 \\
    &= 6(3x - 4)
\end{aligned}
$$

</eg></div>

<div><eg>

Let $h(x) = (5x - 7)^{10}$. Find $h'(x)$.

Again, we can break down $h$ into two different functions: $f$ and $g$. Where:

$$
f(x) = x^{10} \\
g(x) = 5x - 7
$$

Then, $h(x) = f(g(x)) \implies h'(x) = f'(g(x)) \cdot g'(x)$.

$$
\begin{aligned}
    h'(x) &= f'(g(x)) \cdot g'(x) \\
    &= 10(5x - 7)^9 \cdot 5 \\
    &= 50(5x - 7)^9
\end{aligned}
$$


</eg></div>

## The chain and power rule shortcut

<div><def>

Where $h$ and $g$ are differentiable functions, and $n$ is a number:

$$
h(x) = (g(x))^n \implies h'(x) = n \cdot (g(x))^{n-1} \cdot g'(x).
$$

In other words, differentiate it like you would with the power rule. Then, multiply it by the derivative of the "inside part."
</def></div>

<div><eg>

Let $h(x) = (5x - 7)^{10}$. Find $h'(x)$.

Where $g$ is a function such that $g(x) = 5x - 7$ and $n = 10$, we have that:

$$
\begin{aligned}
    h'(x) &= n(g(x))^{n-1} \cdot g'(x) \\
    &= 10(5x - 7)^{10-1} \cdot 5 \\
    &= 50(5x - 7)^9.
\end{aligned}
$$

</eg></div>

<div><eg>

Let $h(x) = (2x^3 + 2x - 1)^4$. Find $h'(x)$.

Where $g$ is a function such that $g(x) = 2x^3 + 2x - 1$ and $n = 4$, we have that:

$$
\begin{aligned}
    h'(x) &= n(g(x))^{n-1} \cdot g'(x) \\
    &= 4(2x^3 + 2x - 1)^{4-1} \cdot (6x^2 + 2) \\
    &= 4(6x^2 + 2)(2x^3 + 2x - 1)^3.
\end{aligned}
$$

</eg></div>

<div><eg>

Let $h(x) = \frac{1}{(3x^2 + 1)^2}$. Find $h'(x)$.

$$
h(x) = \frac{1}{(3x^2 + 1)^2} = (3x^2 + 1)^{-2}
$$

Where $g$ is a function such that $g(x) = 3x^2 + 1$ and $n = -2$, we have that:

$$
\begin{aligned}
    h'(x) &= n(g(x))^{n-1} \cdot g'(x) \\
    &= -2(3x^2 + 1)^{-2-1} \cdot (6x) \\
    &= -12x(3x^2 + 1)^{-3} \\
    &= \frac{1}{(3x^2 + 1)^3}.
\end{aligned}
$$

</eg></div>

<div><eg>

Let $f(x) = \sqrt{8x}$. Find $f'(x)$.

$$
f(x) = \sqrt{8x} = (8x)^{1/2} \\
\begin{aligned}
    \therefore f'(x) &= \frac{1}{2}(8x)^{-1/2} \cdot 8 \\
    &= 4(8x)^{-1/2} \\
    &= \frac{4}{\sqrt{8x}}
\end{aligned}
$$

</eg></div>

<div><eg>

Let $f(x) = (4x^2 - 5)^7 (-2x^2 - 9)^{10}$. Find $f'(x)$.

$$
\begin{aligned}
    u &= (4x^2 - 5)^7 &\implies u' &= 7(8x)(4x^2 - 5)^6 \\
    v &= (-2x^2 - 9)^{10} &\implies v' &= 10(-4x)(-2x^2-9)^{9}
\end{aligned}
\\
\begin{aligned}
    \therefore f'(x) &= u'v + uv' \\
    &= 7(8x)(4x^2 - 5)^6(-2x^2 - 9)^{10} + 10(-4x)(-2x^2-9)^{9}(4x^2 - 5)^7 \\
    &= 56x(4x^2 - 5)^6(-2x^2 - 9)^{10} -40x(-2x^2-9)^{9}(4x^2 - 5)^7 \\
    &= (4x^2 - 5)^6 (-2x^2 - 9)^9 (56x - 40x)
\end{aligned}
$$

</eg></div>

<div><eg>

Let $h(x) = \cos 5x^2$. Find $h'(x)$.

$$
\begin{aligned}
    h'(x) &= (-\sin 5x^2)(10x) \\
    &= -10x\sin 5x^2
\end{aligned}
$$

</eg></div>
