---
    print_background: true
    export_on_save:
        html: true
    puppeteer:
        format: "Letter"
        timeout: 3000
---

$$
    % Differentials d[something]/d[something]
    \gdef\diff#1#2{\frac{\mathrm{d}#1}{\mathrm{d}#2}}
	% Shortcut for dy/dx
    \gdef\dydx{\diff{y}{x}}
	% Shortcut for "not implies"
	\gdef\nimplies{\;\;\;\not\nobreak\!\!\!\!\implies\;}
$$

# 3.7 â€” Derivatives of Inverse Functions

# Inverse functions

Recall that if $f$ is a function. Then, $f^{-1}(x)$ is said to be the **inverse function** of $f(x)$.

<div><important>

$$
f^{-1}(x) \neq \frac{1}{f(x)}
$$

</important></div>

<div><def>

## Inverse function

Let $f$ be a function where $a$ is in the domain of $f$, and $b$ is a number in the range of $f$. Then,

$$
f(a) = b \implies f^{-1}(b) = a.
$$

</def></div>

<div><eg>

Let $f(x) = 3x-5$. Find $f^{-1}(2)$.

$$
\begin{aligned}
    3x-5 &= 2   \\
    3x &= 7 \\
    x &= \frac{7}{3}    \\
    \\
    \therefore f^{-1}(2) &= \frac{7}{3}
\end{aligned}
$$

</eg></div>

## Finding the inverse function

To find the inverse function $f^{-1}(x)$, given a function $f(x)$:

1. Let $y = f(x)$.
2. Solve for $x$.
   The resulting expression for $x$ is the inverse function $f^{-1}(y)$.
3. Rewrite $f^{-1}(y)$ in terms of $x$, by replacing all $y$ in the expression with $x$.

<div><eg>

Let $f(x) = \frac{x+2}{x}$. Find $f^{-1}(x)$.

1. Let $y = f(x)$.
   $$
   y = \frac{x+2}{x}
   $$
2. Solve for $x$.
   $$
   \begin{aligned}
       y &= \frac{x+2}{x}   \\
       xy &= x+2    \\
       xy-x &= 2    \\
       x(y-1) &= 2  \\
       x &= \frac{y-1}{2}
   \end{aligned}
   $$
3. Rewrite the expression with $x$.
   $$
   f^{-1}(x) = \frac{x-1}{2}
   $$

</eg></div>

# Differentiating inverse functions

<div><theo>

## Inverse function theorem

If $f(x)$ is a function such that $f^{-1}(x)$ is its inverse. Then,

$$
(f^{-1})'(x) = \frac{1}{f'(f^{-1}(x))}.
$$

</theo></div>

<div><eg>

Let $f(x) = x^3 - x + 4$. Find $(f^{-1})'(10)$.

$$
f'(x) = 3x^2 - 1    \\
f(2) = 2^3 - 2 + 4 = 10 \\
\\
\therefore f(2) = 10 \implies f^{-1}(10) = 2
$$

By the inverse function theorem, we have that:

$$
\begin{aligned}
    f^{-1}(10) &= \frac{1}{f'(f^{-1}(10))}  \\
    &= \frac{1}{f'(2)}  \\
    &= \frac{1}{3(2)^2 - 1} \\
    &= \frac{1}{11}
\end{aligned}
$$

</eg></div>

# Inverse trigonometric functions

Similar to how we denote inverse functions with $-1$ on the superscript, the notation for trig functions are as follows:

* $\sin^{-1} x$ is the inverse of $\sin x$,
* $\cos^{-1} x$ is the inverse of $\cos x$,
* $\tan^{-1} x$ is the inverse of $\tan x$,
* etc...

<div><important>

$$
\sin^{-1}x \neq \frac{1}{\sin x}
$$

</important></div>

<div><note>

Inverse trig functions may also be referred to with the $\text{arc}$ prefix. For example:

$$
\begin{aligned}
    \sin^{-1}x &= \arcsin x  \\
    \cos^{-1}x &= \arccos x  \\
    \tan^{-1}x &= \arctan x  \\
    & \dots
\end{aligned}
$$

</note></div>

<div><def>

## Derivatives of inverse trigonometric functions

Using the inverse function theorem, we can derive the derivatives of the inverse trig function as follows:

$$
\begin{aligned}
    (\sin^{-1}x)' &= \frac{1}{\sqrt{1-x^2}}  \\
    (\cos^{-1}x)' &= -\frac{1}{\sqrt{1-x^2}}  \\
    (\tan^{-1}x)' &= \frac{1}{1+x^2}  \\
    (\cot^{-1}x)' &= -\frac{1}{1+x^2}  \\
    (\sec^{-1}x)' &= \frac{1}{|x| \sqrt{x^2 - 1}}  \\
    (\csc^{-1}x)' &= -\frac{1}{|x| \sqrt{x^2 - 1}}  \\
\end{aligned}
$$

</def></div>

<div><eg>

Let $f(x) = 6x\cos^{-1}(x)$. Find $f'(x)$.

$$
\begin{aligned}
    u = 6x &\implies u' = 6 \\
    v = \cos^{-1} x &\implies v' = -\frac{1}{\sqrt{1-x^2}}
    \\
    \therefore f'(x) &= u'v + uv' \\
    &= 6\cos^{-1}(x) - \frac{6x}{\sqrt{1 - x^2}} \\
\end{aligned}
$$

</eg></div>

<div><eg>

Let $f(x) = \arcsin(-5x-5)$. Find $f'(x)$.

$$
\begin{aligned}
    f'(x) &= \frac{1}{\sqrt{1-(-5x-5)^2}} \cdot -5 \\
    &= \frac{-5}{\sqrt{1-(-5x-5)^2}}
\end{aligned}
$$

</eg></div>

<div><eg>

Let $f(x) = \tan^{-1}(\cos(5x))$. Find $f'(x)$.

$$
\begin{aligned}
    f'(x) &= \frac{1}{1 + \cos^2(5x)} \cdot \diff{}{x}(\cos(5x)) \\
    &= \frac{1}{1 + \cos^2(5x)} \cdot -\sin(5x) \cdot 5 \\
    &= - \frac{5\sin(5x)}{1 + \cos^2(5x)}
\end{aligned}
$$

</eg></div>
