---
    print_background: true
    export_on_save:
        html: true
    puppeteer:
        format: "Letter"
        timeout: 3000
---

$$
    % Differentials d[something]/d[something]
    \gdef\diff#1#2{\frac{\mathrm{d}#1}{\mathrm{d}#2}}
    % Shortcut for dy/dx
    \gdef\dydx{\diff{y}{x}}
$$

# 3.8 â€” Implicit Differentiation

When dealing with functions of two variables, we have:
* a *dependent variable* (often denoted $y$), and
* an *independent variable* (often denoted $x$).

When we express $y$ in terms of $x$, it is considered to be an **explicit function**.

For example:
$$
y=x^{2} \\
y=\sin{x} \\
y=x^{3}\sin{x}+4x^{2}+\frac{1}{\sqrt{x}}.
$$


Note that $f(x)$ and $y$ are interchangeable. Any expressions above can be expressed with $f(x)$ instead of $y$.

Functions that are *not* defined like ones above are said to be considered to be an **implicit function**.

For example:
$$
	x^{2} + y^{2} = 25.
$$
> This is the equation of a circle centered at the origin with a radius of $5$.

So, how do we find the derivatives of these functions?

* We could try rearranging for $y$:
$$
	x^{2}+y^{2}=25 \\
	y^{2}=25-x^{2} \\
	y=\pm\sqrt{25-x^{2}}.
$$

Now, we get an expression that has a plus-or-minus sign in it. So... how do we differentiate *that*?

**In short, we don't.** It is difficult to convert an implicit function to an explicit function to differentiate.

Instead, we use a technique called **implicit differentiation**.

***

## Notational fuckery
Usually, we use $f'(x)$ to represent the derivative of $f(x)$.
Similarly, $y'$ represents the derivative of $y$.
However, when a function is expressed in terms of $y$, its derivative can also be expressed with the notation: $\dydx$.

The expression $\dydx$ means "the change in $y$ with respect to change in $x$."

## How to: implicit differentiation
If we need to differentiate an implicit function involving $x$ and $y$, do the following:

1. Differentiate both sides of the equation.

<div><note>

When you differentiate $y$, you must multiply it with $\dydx$. This is because $y$ is a function of $x$ (chain rule).

</note></div>

2. Group like terms by rearranging $\dydx$ to the left.
4. Factor and isolate to get the expression in terms of $\dydx$.

<div><eg>

Find the derivative of $x^2+y^2=25$.

1. First, differentiate both sides.
$$
	2x\dydx+2y\dydx=0
$$
2. Then, rearrange and factor.
$$
\begin{aligned}
	2y\dydx&=-2x\\
	\dydx&=\frac{-\cancel{2}x}{\cancel{2}y} \\
	&=-\frac{x}{y}
\end{aligned}
$$
3. As such, we have that the derivative of $x^2+y^2=25$ is $-\frac{x}{y}$.

</eg></div>

<div><eg>

Let $-13x^3+9x^3y^9+y^4=-3$. Find $\dydx$.

Using the sum rule, we can easily differentiate $39x^2$ and $4y^3$.

$$
	-39x^2+\diff{}{x}\diff{}{y}(9x^{39}y)+4y^3\dydx=0 \\
$$

However, notice that we need to use the product rule to differentiate $9x^{39}y$.

Let $u = 9x^{39} \implies u'=351x^{38}$.
Let $v=y \implies v'=\dydx$.
Then:
$$
\begin{aligned}
	\diff{}{x}\diff{}{y} (9x^{39}y) &= u'v+uv' \\
	&= 351x^{38}y+9^{39}\dydx.
\end{aligned}
$$

By substituting the derivative of $9x^{39}y$ back, we have:
$$
	-39x^2+351x^{38}y+9x^{39}\dydx+4y^3\dydx=0.
$$

Isolating $\dydx$ and factoring:
$$
\begin{aligned}
	9x{39}\dydx+4y^3\dydx&=39x^2-351x^{38}y \\
	\dydx(9x^{39}+4x^3)&=39x^2-351x^{38}y
\end{aligned}
$$

Finally, we can get the expression for $\dydx$ by diving by $9x^{39}+4x^3$:
$$
	\dydx=\frac{39x^2-351x^{38}y}{9x^{39}+4x^3}.
$$

</eg></div>
