---
    print_background: true
    export_on_save:
        html: true
    puppeteer:
        format: "Letter"
        timeout: 3000
---

$$
	\gdef\diff#1#2{\frac{\mathrm{d}#1}{\mathrm{d}#2}}
	\gdef\dydx{\diff{y}{x}}
$$

# 3.9 â€” Derivatives of Exponential and Logarithms

# Refreshers

## Exponential function

Recall that **exponential functions** are functions that has the input variable as the exponent. For example:

<div><eg>

$$
	\begin{aligned}
		f(x)&=4^x	\\
		g(x)&=3^{x-2}	\\
		h(x)&=3x^{5x^2-\sin{x}}	\\
		v(x)&=e^x
	\end{aligned}
$$

</eg></div>

## Logarithms

Recall that **logarithms** are the inverse operation of **exponentials**.

<div><eg>

$$
\log_{a}b \iff a^c = b	\\
\log_{2}8 \iff 2^3 = 8
$$

</eg></div>

<div><note>

$$
\ln{x} = \log_{e}x
$$

<div><eg>

Let $e^x=42$. Find $x$.

$$
\begin{aligned}
	e^x&=42	\\
	\ln{e^x}&=\ln{42}	\\
	x&=\ln{42}
\end{aligned}
$$

</eg></div>

</note></div>

# Taking derivatives of exponential functions

Let's start with $e^x$.

If  $f(x)=e^x$. Is $f'(x)=xe^{x-1}$?

* No. $f'(x)\neq xe^{x-1}$.
  The power rule do not apply to exponential functions.
  So, what's the derivative of $e^x$ then?

<div><def>

## Derivative of a natural exponential function

Given a function $f$, if $f(x)=e^x$. Then, $f'(x)=e^x$.

$$
\begin{aligned}
	f(x)=e^x &\implies f'(x)=e^x	\\
	f(x) &= f'(x)
\end{aligned}
$$


<div><note>

For any function $g$, where $f(x)=e^{g(x)}$, the chain rule applies.

$$
f(x)=e^{g(x)} \implies f'(x)=e^{g(x)}\cdot g'(x)
$$


</note></div>

</def></div>

<div><eg>

Let $f(x)=e^{x^2}$. Find $f'(x)$.

$$
\begin{aligned}
	f'(x) &= e^{x^2} \cdot \diff{}{x}x^2	\\
	&= e^{x^2} \cdot 2x	\\
	&= 2xe^{x^2}
\end{aligned}
$$

</eg></div>

<div><eg>

Let $f(x)=8e^{2x+4}$. Find $f'(x)$.

$$
\begin{aligned}
	f'(x) &= 8e^{2x+4} \cdot \diff{}{x}(2x+4)	\\
	&= 8e^{2x+4} \cdot 2	\\
	&= 16e^{2x+4}
\end{aligned}
$$

</eg></div>

<div><eg>

Let $f(x)=xe^{2x}$. Find $f'(x)$.

Notice that the product rule applies here since $x$ is being multiplied by the exponential part, $e^{2x}$.

$$
\begin{aligned}
	f'(x) &= \diff{}{x}(x)\cdot e^{2x} + x\cdot\diff{}{x}(e^{2x})	\\
	&= e^{2x} + x\cdot 2e^{2x}	\\
	&= e^{2x}(1+2x)
\end{aligned}
$$

</eg></div>

<div><eg>

Let $y = \frac{e^{x^2}}{x}$. Find $y'$.

Similarly, the quotient rule appiles here.

$$
\begin{aligned}
    u &= e^{x^2} &\implies u' &= 2xe^{x^2}    \\
    v &= x &\implies v' &= 1
\end{aligned}
\\
\begin{aligned}
    \therefore y' &= \frac{u'v-uv'}{v^2}    \\
    &= \frac{2xe^{x^2}\cdot x - e^{x^2}}{x^2}   \\
    &= \frac{e^{x^2}(2x^2 - 1)}{x^2}
\end{aligned}
$$

</eg></div>

<div><eg>

Let $f(x) = e^{\tan{2x}}$. Find $f'(x)$.

$$
\begin{aligned}
    f'(x) &= e^{\tan{2x}} \cdot \diff{}{x}(\tan{2x})    \\
    &= e^{\tan{2x}} \cdot \sec^2{(2x)} \cdot 2    \\
    &= 2e^{\tan{2x}}\sec^2{2x}
\end{aligned}
$$

</eg></div>

# Taking derivatives of logarithmic functions

Let's start with $\ln{x}$.

* Let $y = \ln{x}$. Find $y'$.
  To differentiate with respect to $x$, we start by rearranging for $x$.

  $$
  \begin{aligned}
    y &= \ln{x}  \\
    e^y &= e^{\ln{x}}  \\
    x &= e^y
  \end{aligned}
  $$

  Then, by implicit differentiation, we have that:
  $$
  \begin{aligned}
    \diff{}{x}(x) &= \dydx{e^y}   \\
    1 &= \dydx{e^y}.
  \end{aligned}
  $$

  Rearranging for $\dydx$, we have the following expression:
  $$
  \dydx = \frac{1}{e^y}.
  $$

  Since $x=e^y$, we can substitute $x$ into the expression above to get the derivative with respect to $x$.
  $$
  \dydx = y' = \frac{1}{x}
  $$

<div><def>

## Derivative of a natural logarithmic function

$$
f(x)=\ln{x} \implies f'(x)=\frac{1}{x}
$$

<div><note>

For any function $g$, where $f(x)=\ln{g(x)}$, the chain rule applies.

$$
f(x)=\ln{g(x)} \implies f'(x)=\frac{1}{g(x)}\cdot g'(x) = \frac{g'(x)}{g(x)}
$$

</note></div>

</def></div>

<div><eg>

Let $f(x)=\ln{x^3}$. Find $f'(x)$.

$$
\begin{aligned}
    f'(x) &= \frac{1}{x^3} \cdot 3x^2  \\
    &= \frac{3\cancel{x^2}}{x^{\cancel{3}}} \\
    &= \frac{3}{x}
\end{aligned}
$$


</eg></div>

<div><eg>

Let $f(x) = \ln(x^4+3x-4)$. Find $f'(x)$.

$$
\begin{aligned}
    f'(x) &= \frac{1}{x^4 + 3x -4} \cdot \diff{}{x}(x^4 + 3x -4)    \\
    &= \frac{1}{x^4 + 3x -4} \cdot 4x^3 + 3    \\
    &= \frac{4x^3 + 3}{x^4 + 3x -4}
\end{aligned}
$$

</eg></div>

<div><eg>

Let $f(x)=6x^7\ln x^2$. Find $f'(x)$.

$$
\begin{aligned}
    u = 6x^7 &\implies u' = 42x^6    \\
    v = \ln x^2 &\implies v'=\frac{2x}{x^2}  \\
\end{aligned}
\\
\begin{aligned}
    \therefore f'(x) &= u'v + uv'    \\
    &= 42x^6 \ln(x^2) + 6x^7 \cdot \frac{2x}{x^2}   \\
    &= 42x^6 \ln(x^2) + 12x^6   \\
    &= 6x^6(7\ln(x^2) + 2)
\end{aligned}
$$

</eg></div>

<div><eg>

Let $f(x)= \ln(\cos 5x)$. Find $f'(x)$.

$$
\begin{aligned}
    f'(x) &= \frac{1}{\cos 5x} \cdot \diff{}{x}(\cos 5x)    \\
    &= \frac{1}{\cos 5x} \cdot -5\sin 5x    \\
    &= -\frac{5\sin 5x}{\cos 5x}    \\
    &= -5\tan 5x
\end{aligned}
$$



</eg></div>
