---
    print_background: true
    export_on_save:
        html: true
    puppeteer:
        format: "Letter"
        timeout: 3000
---

$$
    % Differentials d[something]/d[something]
    \gdef\diff#1#2{\frac{\mathrm{d}#1}{\mathrm{d}#2}}
    % Shortcut for dy/dx
    \gdef\dydx{\diff{y}{x}}
    % Differential letter "d" with a thin space before it
    \gdef\dd{\mathop{}\!\mathrm{d}}
    % Shortcut for not implies
    \gdef\nimplies{\;\;\;\not\nobreak\!\!\!\!\implies\;}
    % Shortcuts for extended brackets
    \gdef\({\left(} \gdef\){\right)}
    % Shortcut for real number symbol
    \gdef\R{\mathbb{R}}
$$

# 4.10 â€” Antiderivatives

We've spent a lot of time differentiating functions. We now ask the opposite question: if we start with a derivative, can we find the original function?

# The reverse of differentiation

<div><def>

A function $F$ is an **antiderivative** of the function $f$ if
$$
F'(x) = f(x)
$$

for all $x$ in the domain of $f$.

</def></div>

For example, let $f(x)=3x^2$. Find the antiderivative of $f(x)$.

If our function has a power of $2$, then we know that its antiderivative must have a power of $2+1$ from the power rule.

So far, we have that the antiderivative of $f$ is $F(x)=x^3$.

And using the definition, we see that
$$
F(x) = x^3 \implies F'(x) = 3x^2.
$$

However, we cannot conclude that $F(x)=x^3$ is the antiderivative of $f$. This is because there may be a constant in the antiderivative that produces the same function. For example, $x^3+1$ is also an antiderivative of $3x^2$, and so is $x^3 + \sqrt{\pi}$.
$$
\diff{}{x}(x^3+1)=\diff{}{x}(x^3+\sqrt{\pi})=3x^2
$$

As we can see, since the derivative of any constant $c$ is zero, we must consider that in our expression for the antiderivative.

As such, we conclude that the antiderivative of $f(x)=3x^2$ is $F(x)=x^3+c$.

<div><eg>

Let $f(x)=4x$. Find the antiderivative $F(x)$.

$$
f(x) = 4x \implies F(x) = 2x^2 + c
$$

Again, to check our assumption, we can differentiate $F$ where $c$ is some constant.
$$
F(x) = 2x^2 + c \implies F'(x) = 4x
$$

As we can see, differentiating the antiderivative gives us $f$.

As such, the antiderivative is $F(x)=2x^2+c$.

</eg></div>

<div><eg>

Let $f(x) = 7x^3$. Find the antiderivative $F(x)$.

$$
f(x) = 7x^3 \implies F(x)=\frac{7}{4}x^4+c
$$

</eg></div>

<div><theo>

## Reverse power rule

We can apply the power rule of differentiation backwards in order to find its antiderivative.

If $f$ is a function such that $f(x)=ax^n$, where $a$ and $n$ are  constants such that $n\neq-1$.

Then, the antiderivative of $f$ is
$$
F(x) = \frac{ax^{n+1}}{n+1}+c
$$

where $c$ is a constant.

</theo></div>

<div><eg>

Let $f(x)=-8x^3$. Find the antiderivative $F(x)$.

Using the reverse power rule, we have that
$$
\begin{aligned}
    F(x) &= \frac{-8x^{3+1}}{3+1}+c \\[1em]
    &= \frac{-8x^4}{4}+c \\[1em]
    &= -2x^4+c.
\end{aligned}
$$

</eg></div>

<div><eg>

Let $f(x) = \sqrt{x}$. Find the antiderivative $F(x)$.

Rewrite $\sqrt{x}$ and use the reverse power rule.
$$
f(x) = \sqrt{x} = x^\frac{1}{2}\\
\begin{aligned}
    F(x) &= \frac{x^\frac{3}{2}}{\frac{3}{2}} + c \\[1.3em]
    &= \frac{2}{3}x^\frac{3}{2} + c \\[1em]
    &= \frac{2}{3}\sqrt{x^3} + c
\end{aligned}
$$

</eg></div>

<div><eg>

Let $f(x) = \frac{4}{x^2}$. Find the antiderivative $F(x)$.

$$
f(x) = \frac{4}{x^2} = 4x^{-2} \\
\begin{aligned}
    F(x) &= \frac{4x^{-1}}{-1}+c \\[1em]
    &= -4x^{-1}+c \\[.5em]
    &= -\frac{4}{x}+c
\end{aligned}
$$
</eg></div>

## Other nasty antiderivatives

<div><eg>

Let $f(x)=\sin x$. Find the antiderivative.

$$
f(x)=\sin x \implies F(x) = -\cos(x)+c
$$

</eg></div>

<div><eg>

Let $f(x)=5\sec^2(x)$. Find the antiderivative.

$$
f(x)=5\sec^2(x) \implies F(x)=5\tan x + c
$$

</eg></div>

<div><eg>

Let $f(x)=e^x$. Find the antiderivative.

$$
f(x) = e^x \implies F(x) = e^x + c
$$

</eg></div>

<div><eg>

Let $f(x) = x^{-1}$. Find the antiderivative.

<div><important>

Note that we cannot apply the reverse power rule here.
$$
F(x)=\frac{x^{-1+1}}{-1+1}=\frac{x^0}{0}=\frac{1}{0}
$$

</important></div>

This is a special case where we cannot apply the reverse power rule (where the power is $-1$).

Instead, recall that $\diff{}{x}\ln x = \frac{1}{x}$.
$$
f(x) = x^{-1} = \frac{1}{x} \implies F(x) = \ln |x| + c
$$

</eg></div>

# Notational fuckery

There is a universal notation used for antiderivatives. It is known as the **indefinite integrals**, and it uses a symbol called an **integral sign**.

<div><def>

Given a function $f$, the **indefinite integral** of $f$, denoted
$$
\int f(x)\dd x
$$
is the most general antiderivative of $f$.

If $F$ is an antiderivative of $f$, then
$$
\int f(x)\dd x = F(x) + c.
$$

* The expression $f(x)$ is called the *integrand*.
* $x$ is called the *variable of integration*.
* And the expression $\int f(x)\dd x$ is called "the indefinite integral of $f$."

</def></div>

<div><eg>

Compute $\int2x\dd x$.

Again, all this means is that it is asking for the antiderivative of $2x$.
$$
\int2x\dd x = \frac{2x^2}{2} + c = x^2 + c
$$

</eg></div>

<div><eg>

Compute $\int(x^3+5x^2+e^x)\dd x$.

Just like when we differentiate a sum, we can integrate them separately --- but don't forget the $+c$!
$$
\begin{aligned}
    \int(x^3+5x^2+e^x)\dd x &= \frac{x^4}{4}+\frac{5x^3}{3}+e^x+c \\
    &= \frac{1}{4}x^4 + \frac{5}{3}x^3 + e^x + c
\end{aligned}
$$

</eg></div>

<div><theo>

With the new fancy notation, we can rewrite our [reverse power rule](#reverse-power-rule).

## Power rule for integrals

For $n\neq-1$,
$$
\int x^n \dd x = \frac{x^{n+1}}{n+1}+c
$$

where $c$ is a constant.

</theo></div>


# Initial-value problems

Normally, when finding an antiderivative, we include a $c$ to indicate an unknown constant. But, if we have additional information about our function, we can figure out what these constants are.

<div><eg>

Let $f'(x)=x^{-3}$. Find $f(x)$ where $f(1)=1$.

$$
f'(x)=x^{-3} \implies f(x) =-\frac{1}{2x^2}+c
$$

Since we are given that $f(1)=1$, we can use this to solve for $c$.
$$
-\frac{1}{2(1)^2}+c=1 \\
\therefore c = \frac{3}{2}
$$

As such, we have that
$$
f(x) = -\frac{1}{2x^2}+\frac{3}{2}.
$$

</eg></div>

<div><eg>

Let $f''(x)=8x^5-4x^3+6x-7+e^x$.
Assume $f'(0)=f(0)=0$. Find $f(x)$.

Notice that we are given the second derivative of $f$, as such we must find the antiderivative twice, and also use the given values to find the unknown constants for each steps.

$$
f''(x)=8x^5-4x^3+6x-7+e^x \implies f'(x) = \frac{4}{3}x^6-x^4+3x^2-7x+e^x+c_1
$$

Since we are given that $f'(0)=0$, we can use this information to solve for $c_1$.
$$
\frac{4}{3}(0)^6-(0)^4+3(0)^2-7(0)+e^0+c_1=0 \\
\therefore c_1 = -1
$$

As such, we have that the first derivative is
$$
f'(x) = \frac{4}{3}x^6-x^4+3x^2-7x+e^x-1.
$$

Now, we find the original function by doing the same thing again.
$$
f'(x) = \frac{4}{3}x^6-x^4+3x^2-7x+e^x-1 \\
\implies f(x) = \frac{4}{21}x^7-\frac{1}{5}x^5+x^3-\frac{7}{2}x^2+e^x-x+c_0
$$

Again, we know that $f(0)=0$, so we use it to solve for $c_0$.
$$
\frac{4}{21}(0)^7-\frac{1}{5}(0)^5+(0)^3-\frac{7}{2}(0)^2+e^0-0+c_0 = 0 \\
\therefore c_0=-1
$$

<div><important>

$$
c_1=-1 \nimplies c_0=c_1=-1
$$

Note that in this case, $c_0 = c_1$. However, this may not necessarily be the case.

We will need to use the given information to find the different values of $c$. As such, we may not assume that $c_0=-1$ simply because $c_1=-1$.

</important></div>

And so, finally we have that the original function is
$$
f(x) = \frac{4}{21}x^7-\frac{1}{5}x^5+x^3-\frac{7}{2}x^2+e^x-x-1.
$$

</eg></div>
