---
    print_background: true
    export_on_save:
        html: true
    puppeteer:
        format: "Letter"
        timeout: 3000
---

$$
    % Differentials d[something]/d[something]
    \gdef\diff#1#2{\frac{\mathrm{d}#1}{\mathrm{d}#2}}
    % Shortcut for dy/dx
    \gdef\dydx{\diff{y}{x}}
    % Shortcut for not implies
    \gdef\nimplies{\;\;\;\not\nobreak\!\!\!\!\implies\;}
    % Shortcuts for extended brackets
    \gdef\({\left(} \gdef\){\right)}
    % Shortcut for real number symbol
    \gdef\R{\mathbb{R}}
$$

# 4.8 — L’Hôpital’s Rule

# Recap: limit theory

Recall that if:
$$
\lim_{x\to a}f(x) = L_1 \\
\lim_{x\to a}g(x) = L_2 \neq 0.
$$

Then,
$$
\lim_{x\to a}\frac{f(x)}{g(x)} = \frac{L_1}{L_2}.
$$

But... what if $L_1, L_2 = 0$? Like
$$
\lim_{x\to2}\frac{x^2-4}{x-2}.
$$

Evaluating the limits of the numerator and denominator yields zero for both.
$$
\lim_{x\to2}(x^2-4) = \lim_{x-2}(x^2-4) = 0
$$

Which then gives us an indeterminate form $\frac{0}{0}$. Previously, we learned that we can factor the expression in order to evaluate the limit.
$$
\lim_{x\to2}\frac{x^2-4}{x-2} = \lim_{x\to2}\frac{\cancel{(x-2)}(x+2)}{\cancel{x-2}} = 4
$$

However, we can't do the same with expressions like
$$
\lim_{x\to0}\frac{\sin x}{x}
$$

because
$$
\lim_{x\to0}\sin0 = \lim_{x\to0}x = 0
$$

and evaluating them by plugging them in would give us $\frac{0}{0}$, which is indeterminate.

We can get around this using **L’Hôpital’s rule**, which uses local linear approximations to evaluate limits that produces indeterminate forms lke the ones above and many more.

# L’Hôpital’s rule

<div><theo>

## L’Hôpital’s rule ($\bold{0/0}$ form)

Suppose $f$ and $g$ are differentiable functions over an open interval containing $a$, except possibly **at** $a$. If $\displaystyle\lim_{x\to a} f(x) = \lim_{x\to a} g(x) = 0$, then

$$
\lim_{x\to a}\frac{f(x)}{g(x)} = \lim_{x\to a}\frac{f'(x)}{g'(x)},
$$

assuming the limit on the right exists or is $\infty$ or $-\infty$. This also holds if the limit is infinite where $a=\infty$ or $a=-\infty$, or the limit is one-sided.

</theo></div>

<div><eg>

Evaluate $\displaystyle\lim_{x\to a}\frac{x^2-4}{x-2}$.

First, check that L’Hôpital’s rule actually applies, i.e., that the limit of the numerator *and* denominator is zero.
$$
\lim_{x\to2}(x^2-4) = 2^2-4 = 0 = \lim_{x\to2}(x-2) = 2-2
$$

Since $x^2-4\to0$ and $x-2\to0$, we can apply L’Hôpital’s rule.
$$
\begin{aligned}
    \lim_{x\to2}\frac{x^2-4}{x-2} &= \lim_{x\to2}\frac{\diff{}{x}(x^2-4)}{\diff{}{x}(x-2)} \\[1.5em]
    &= \lim_{x\to2}\frac{2x}{1} \\[1em]
    &= 4
\end{aligned}
$$


</eg></div>

<div><eg>

Now, let's try using L’Hôpital’s rule to evaluate $\displaystyle\lim_{x\to0}\frac{\sin x}{x}$.

Again, checking if both $\sin x\to0$ and $x\to0$.
$$
\lim_{x\to0}(\sin x) = \sin0 = 0 = \lim_{x\to0}x = 0
$$

Sure enough, they are. And so applying L’Hôpital’s rule gives us:
$$
\lim_{x\to0}\frac{\sin x}{x} = \lim_{x\to0}\frac{\cos x}{1}=\cos0=1
$$

Thus, $\displaystyle\lim_{x\to0}\frac{\sin x}{x} = 1$. Much easier!

</eg></div>

<div><eg>

Evaluate $\displaystyle\lim_{x\to\infty}\frac{e^{\frac{1}{x}}-1}{\frac{1}{x}}$.

First, check if the rule applies.
$$
\lim_{x\to\infty}\frac{e^{\frac{1}{x}}-1}{\frac{1}{x}} = \frac{1-1}{0} = \frac{0}{0}
$$

It does, so we apply the rule.
$$
\begin{aligned}
    \lim_{x\to\infty}\frac{e^{\frac{1}{x}}-1}{\frac{1}{x}} &= \lim_{x\to\infty}\frac{\diff{}{x}(e^{\frac{1}{x}}-1)}{\diff{}{x}\(\frac{1}{x}\)} \\[1.5em]
    &= \lim_{x\to\infty}\frac{-\frac{e^{\frac{1}{x}}}{x^2}}{-\frac{1}{x^2}} \\[1.5em]
    &= \lim_{x\to\infty}\frac{\cancel{x^2}e^\frac{1}{x}}{\cancel{x^2}} \\[1em]
    &= \lim_{x\to\infty}e^\frac{1}{x} \\
    &= 1
\end{aligned}
$$

</eg></div>

We can also use L’Hôpital’s rule when we get get an indeterminate form like $\frac{\infty}{\infty}$.

<div><theo>

## L’Hôpital’s rule ($\bold{\infty/\infty}$ form)

Suppose $f$ and $g$ are differentiable functions over an open interval containing $a$, except possibly **at** $a$. If $\displaystyle\lim_{x\to a} f(x) = \lim_{x\to a} g(x) = \infty$ or $\displaystyle\lim_{x\to a} f(x) = \lim_{x\to a} g(x) = -\infty$, then

$$
\lim_{x\to a}\frac{f(x)}{g(x)} = \lim_{x\to a}\frac{f'(x)}{g'(x)},
$$

assuming the limit on the right exists or is $\infty$ or $-\infty$. This also holds if the limit is infinite where $a=\infty$ or $a=-\infty$, or the limit is one-sided.

</theo></div>

<div><eg>

Evaluate $\displaystyle\lim_{x\to\infty}\frac{3x+5}{2x+1}$.

We could divide the numerator and denominator by $x$ to find the limit. Or, we can use L’Hôpital’s rule.

First, check if L’Hôpital’s rule applies here.
$$
\lim_{x\to\infty}\frac{3x+5}{2x+1} \implies \frac{\displaystyle\lim_{x\to\infty}3x+5}{\displaystyle\lim_{x\to\infty}2x+1} = \frac{\infty}{\infty}
$$

Then, applying the rule, we have that:
$$
\begin{aligned}\lim_{x\to\infty}\frac{3x+5}{2x+1} &= \lim_{x\to\infty}\frac{\diff{}{x}\(3x+5\)}{\diff{}{x}\(2x+1\)} \\[1.5em]
&= \lim_{x\to\infty}\frac{3}{2} \\[1em]
&= \frac{3}{2}.
\end{aligned}
$$

</eg></div>

<div><eg>

Evaluate $\displaystyle\lim_{x\to\infty}\frac{2x+3}{11x^2-7x+4}$.

Clearly, the limits of both numerator and denominator is $\infty$. As such, we apply the rule.

$$
\begin{aligned}
    \lim_{x\to\infty}\frac{2x+3}{11x^2-7x+4} &= \lim_{x\to\infty}\frac{\diff{}{x}(2x+3)}{\diff{}{x}(11x^2-7x+4)} \\[1em]
    &= \lim_{x\to\infty}\frac{2}{22x-7} \\[1em]
    &= 0
\end{aligned}
$$


</eg></div>

<div><eg>

Evaluate $\displaystyle\lim_{x\to0}\frac{e^x-x-1}{7x^2}$.

Again, checking if the rule applies, we have that:
$$
\lim_{x\to0}\frac{e^x-x-1}{7x^2} = \lim_{x\to0}\frac{1-0-1}{0} = \frac{0}{0}.
$$

Applying L’Hôpital’s rule, we have:
$$
\begin{aligned}
    \lim_{x\to0}\frac{e^x-x-1}{7x^2} &= \lim_{x\to0}\frac{\diff{}{x}(e^x-x-1)}{\diff{}{x}(7x^2)} \\[1em]
    &= \lim_{x\to0}\frac{e^x-1}{14x}.
\end{aligned}
$$

If we try and evaluate the limit, we'll find that the result we get is still indeterminate!
$$
\lim_{x\to0}\frac{e^x-1}{14x} = \frac{1-1}{14\cdot0} = \frac{0}{0}
$$

As such, we can apply L’Hôpital’s rule **again**.
$$
\begin{aligned}
    \lim_{x\to0}\frac{e^x-1}{14x} &= \lim_{x\to0}\frac{e^x}{14} \\[1em]
    &= \frac{1}{14}
\end{aligned}
$$

And so, we have that $\displaystyle\lim_{x\to0}\frac{e^x-x-1}{7x^2} = \frac{1}{14}$.

</eg></div>

## Using L’Hôpital’s rule for other indeterminate forms

L’Hôpital’s rule can also be used to evaluate expressions where you have other indeterminate forms, such as:
$$
\begin{array}{c}
    0\cdot\infty, & \infty-\infty, & 1^\infty, & 0^0,\text{ and} & \infty^0.
\end{array}
$$

But, we must first manipulate the expression to be $\frac{0}{0}$ or $\frac{\infty}{\infty}$ in order to use L’Hôpital’s rule.

<div><eg>

Evaluate $\displaystyle\lim_{x\to0^+}(x\cdot\ln x)$.

Using the limit laws, we have that:
$$
\lim_{x\to0^+}(x\cdot\ln x) = \lim_{x\to0^+}(x)\lim_{x\to0^+}\ln(x) = 0\cdot\infty.
$$

Here, we can't apply L’Hôpital’s rule yet. However, we can manipulate it in such a way that one of the L’Hôpital’s rule cases applies.
$$
\lim_{x\to0^+}(x\cdot\ln x) = \lim_{x\to0^+}\frac{\ln x}{\frac{1}{x}}
$$

Then, we have that:
$$
\begin{aligned}
    \lim_{x\to0^+}\frac{\ln x}{\frac{1}{x}} &= \lim_{x\to0^+}\frac{\diff{}{x}(\ln x)}{\diff{}{x}\(\frac{1}{x}\)} \\[1.5em]
    &= \lim_{x\to0^+} \frac{\frac{1}{x}}{-\frac{1}{x^2}}\ \\[1em]
    &= \lim_{x\to0^+}(-x) \\
    &= 0.
\end{aligned}
$$

As such, we conclude that $\displaystyle\lim_{x\to0^+}\frac{\ln x}{\frac{1}{x}} = 0$.

</eg></div>

<div><eg>

Evaluate $\displaystyle\lim_{x\to\frac{\pi}{2}}5\cos(-7x)\sec(9x)$.

Here, we have that:
$$
\lim_{x\to\frac{\pi}{2}}5\cos(-7x)\sec(9x) = \lim_{x\to\frac{\pi}{2}}(5)\lim_{x\to\frac{\pi}{2}}\cos(-7x)\lim_{x\to\frac{\pi}{2}}\sec(9x) \\
= 5 \cdot 0 \cdot \infty.
$$

One way we can manipulate the expression is writing $\sec9x$ as $\frac{1}{\cos9x}$.
$$
\begin{aligned}
    \lim_{x\to\frac{\pi}{2}}5\cos(-7x)\sec(9x) &= \lim_{x\to\frac{\pi}{2}}5\cos(-7x)\cdot\frac{1}{\cos 9x} \\[1em]
    &= \lim_{x\to\frac{\pi}{2}}\frac{5\cos(-7x)}{\cos9x} \\[1em]
    &=\frac{5\cdot1}{1} \\[1em]
    &= 5
\end{aligned}
$$

And so, we have that $\displaystyle\lim_{x\to\frac{\pi}{2}}5\cos(-7x)\sec(9x) = 5$.

</eg></div>


## "The limit does not exist!"
Compute $\displaystyle\lim_{x\to0}\frac{\ln(1-x)-\sin x}{1-\cos^2x}$.

Using the trig identity $\cos^2+\sin^2=1$, we can rewrite the limit.
$$
\begin{aligned}
    \lim_{x\to0}\frac{\ln(1-x)-\sin x}{1-\cos^2x} &=  \lim_{x\to0}\frac{\ln(1-x)-\sin x}{\sin^2x}
\end{aligned}
$$

Let's try to find the limit by direct substitution.
$$
\begin{aligned}
    \lim_{x\to0}\frac{\ln(1-x)-\sin x}{\sin^2x} &= \frac{\ln(1-0)-\sin 0}{\sin^20} \\[1em]
    &= \frac{0}{0}
\end{aligned}
$$

We get the indeterminate form $0/0$, so we can use L’Hôpital’s rule.
$$
\begin{aligned}
    \lim_{x\to0}\frac{\ln(1-x)-\sin x}{\sin^2x} &= \lim_{x\to0}\frac{\diff{}{x}(\ln(1-x)-\sin x)}{\diff{}{x}(\sin^2x)} \\[2em]
    &= \lim_{x\to0}\frac{\frac{-1}{1-x}-\cos x}{2\sin x\cos x}
\end{aligned}
$$

Then, using the identity $\sin(2x)=2\sin x\cos x$, we rewrite the limit again.
$$
\begin{aligned}
    \lim_{x\to0}\frac{\frac{-1}{1-x}-\cos x}{2\sin x\cos x} &= \lim_{x\to0}\frac{\frac{-1}{1-x}-\cos x}{\sin(2x)}
\end{aligned}
$$

Using limit laws, we evaluate the limit of the numerator and denominator separately.
$$
\lim_{x\to0}\frac{\frac{-1}{1-x}-\cos x}{\sin(2x)} = \lim_{x\to0}\(\frac{-1}{1-x}-\cos x\) \cdot \lim_{x\to0}\frac{1}{\sin(2x)}
$$



